src/Dafny/examples/fs/block_fs.dfy
@@ -49,6 +49,7 @@ module BlockFs
     ensures fs.ValidQ()
     ensures block_data(fs.data) == map ino: Ino {:trigger} :: InodeData.zero
     ensures fs.metadata == map ino: Ino {:trigger} :: Inode.Meta(0, Inode.FileType)
+    ensures fs.inode_owner() == map ino: Ino {:trigger} :: Fs.None
   {
     fs := new IndFilesys.Init(d);
     reveal inode_blocks();
