src/Dafny/examples/fs/dir_fs.dfy
@@ -1,0 +1,73 @@
+include "byte_fs.dfy"
+include "dirent.dfy"
+
+module DirFs
+{
+  import opened Machine
+  import opened ByteSlice
+  import opened Fs
+  import opened FsKinds
+  import opened JrnlTypes
+  import opened JrnlSpec
+
+  import opened DirEntries
+  import opened ByteFs
+
+  import C = Collections
+
+  datatype File =
+    | ByteFile(data: seq<byte>)
+    | DirFile(dir: Directory)
+
+  class DirFilesys
+  {
+    // external abstract state
+    //
+    // domain consists of allocated inodes
+    ghost var data: map<Ino, File>
+
+    // internal state, tracking exactly how directories are encoded
+    // domain is just the inodes that are allocated directories
+    ghost var dirents: map<Ino, Dirents>
+    const fs: ByteFilesys<()>
+
+    const Repr: set<object> := {this} + fs.Repr
+
+    static predicate alloc_ino_dom<T>(inode_owner: map<Ino, Option<()>>, m: map<Ino, T>)
+      requires ino_dom(inode_owner)
+    {
+      forall ino:Ino :: ino in m <==> inode_owner[ino].Some?
+    }
+
+    predicate ValidDomains()
+      requires fs.Valid()
+      reads Repr
+    {
+      && alloc_ino_dom(fs.fs.inode_owner(), data)
+      && forall ino:Ino :: ino in dirents <==>
+        (fs.fs.inode_owner()[ino].Some? && fs.inode_types()[ino].DirType?)
+    }
+
+    predicate ValidDirents()
+      reads Repr
+    {
+      // relate fs.data() to dirents
+      true
+    }
+
+    predicate Valid()
+      reads Repr
+    {
+      && fs.Valid()
+      && ValidDomains()
+    }
+
+    constructor Init(d: Disk)
+      ensures Valid()
+    {
+      fs := new ByteFilesys.Init(d);
+      dirents := map[];
+      data := map[];
+    }
+  }
+}
