src/Dafny/examples/fs/indirect_fs.dfy
@@ -203,12 +203,14 @@ module IndFs
       ensures fs.quiescent()
       ensures data == imap pos: Pos | pos.idx.data? :: block0
       ensures metadata == map ino: Ino {:trigger} :: Inode.Meta(0, Inode.FileType)
+      ensures inode_owner() == map ino: Ino {:trigger} :: None
     {
       this.fs := new Filesys.Init(d);
       this.to_blkno := imap pos: Pos {:trigger} :: 0 as Blkno;
       this.data := imap pos: Pos | pos.idx.data? :: block0;
       this.metadata := map ino: Ino {:trigger} :: Inode.Meta(0, Inode.FileType);
       new;
+      assert ValidBasics() by { reveal fsValid(); }
       IndBlocks.to_blknos_zero();
       reveal ValidPos();
       reveal ValidInodes();
